Proof/AbstractDetectsCycle.lean
@@ -1,0 +1,44 @@
+import Proof.Semantics
+import Proof.Stack
+import Proof.Analysis
+import Proof.CorrectnessRelation
+import Mathlib.Tactic.Set
+import Proof.AccessImpliesDep
+import Proof.StackDepChain
+import Proof.PartialOnStack
+
+namespace Proof
+
+theorem abstract_detects_cycle {L : Program} {G Gₘ: GlobName} {S : Stack}
+  {σ : Sigma} {E : ECtx} {H : Heap} {Γ : GTable} {i : Idx} {u₁ u₂ : GVal}
+  (hσ : FixPoint σ L)
+  (hrun : Star L (.mk (fun _ => none) (fun _ => none) List.nil (Expr.gproj Gₘ Idx.one))
+      (.mk H Γ S (E.plug (Expr.gproj G i))))
+  (hG : Γ G = (GEntry.mk u₁ u₂)) (hnone: u₁ = none ∨ u₂ = none) :
+  G ∈ Dep σ L G := by
+
+  have hGOnStack : inGlobals G S := (partially_init_obj_on_stack hrun hG hnone)
+  have hinv : Inv σ L (.mk H Γ S (E.plug (Expr.gproj G i))) := inv_preservation hσ hrun
+  have hrinv: REInv σ L (.mk H Γ S (E.plug (Expr.gproj G i))) := REInv.preservation hσ hrun
+  have hsd : StackDep σ L (.mk H Γ S (E.plug (Expr.gproj G i))) := stack_dep_run hσ hrun
+
+  obtain ⟨f, hfS, hfG⟩ := hGOnStack
+
+  obtain ⟨ifr, cfs, r, hti⟩ := Stack.hasInit_of_glob hfS hfG
+  obtain ⟨Gₜ, hGₜ⟩ := Frame.glob_of_notCall (Stack.topInit_notCall hti)
+  have htiG : Stack.TopInit S Gₜ := by
+    intro i' cfs' r' h
+    rw [hti] at h
+    simp only [Option.some.injEq, Prod.mk.injEq] at h
+    obtain ⟨rfl, -, -⟩ := h
+    exact hGₜ
+
+  have hGInDepGₜ : G ∈ Dep σ L Gₜ := acc_implies_dep hti htiG hinv hrinv
+
+  obtain ⟨pre, suf, hS⟩ := List.append_of_mem hfS
+
+  rcases StackDep.topInit_dep hsd hti hGₜ hS hfG with rfl | hGₜInDepG
+  · exact hGInDepGₜ
+  · exact DepJ.trans hGₜInDepG hGInDepGₜ
+
+end Proof
